added pyhon code and test

main-py/Lem.py
@@ -1,0 +1,13 @@
+import sys
+from typing import Callable, Any, TypeVar, NamedTuple
+from math import floor
+from itertools import count
+
+import module_ as module_
+import _dafny as _dafny
+import System_ as System_
+import Type as Type
+import Property as Property
+
+# Module: Lem
+
