main-py/Operations.py
@@ -1,0 +1,128 @@
+import sys
+from typing import Callable, Any, TypeVar, NamedTuple
+from math import floor
+from itertools import count
+
+import module_ as module_
+import _dafny as _dafny
+import System_ as System_
+import Type as Type
+import Property as Property
+import Lem as Lem
+
+# Module: Operations
+
+class default__:
+    def  __init__(self):
+        pass
+
+    @staticmethod
+    def rotateLeft(h):
+        result: Type.Rb__tree = Type.Rb__tree.default()()
+        d_0_new__h_: Type.Rb__tree
+        d_0_new__h_ = Type.Rb__tree_Node(Type.Color_Red(), (h).key, (h).left, ((h).right).left)
+        result = Type.Rb__tree_Node((h).color, ((h).right).key, d_0_new__h_, ((h).right).right)
+        return result
+        return result
+
+    @staticmethod
+    def rotateRight(h):
+        result: Type.Rb__tree = Type.Rb__tree.default()()
+        d_0_new__h_: Type.Rb__tree
+        d_0_new__h_ = Type.Rb__tree_Node(Type.Color_Red(), (h).key, ((h).left).right, (h).right)
+        result = Type.Rb__tree_Node((h).color, ((h).left).key, ((h).left).left, d_0_new__h_)
+        return result
+        return result
+
+    @staticmethod
+    def flip__color(h):
+        result: Type.Rb__tree = Type.Rb__tree.default()()
+        d_0_new__left__nodeColor_: Type.Color
+        if (((h).left).color) == (Type.Color_Red()):
+            d_0_new__left__nodeColor_ = Type.Color_Black()
+        elif True:
+            d_0_new__left__nodeColor_ = Type.Color_Red()
+        d_1_new__left_: Type.Rb__tree
+        d_1_new__left_ = Type.Rb__tree_Node(d_0_new__left__nodeColor_, ((h).left).key, ((h).left).left, ((h).left).right)
+        d_2_new__right__nodeColor_: Type.Color
+        if (((h).right).color) == (Type.Color_Red()):
+            d_2_new__right__nodeColor_ = Type.Color_Black()
+        elif True:
+            d_2_new__right__nodeColor_ = Type.Color_Red()
+        d_3_new__right_: Type.Rb__tree
+        d_3_new__right_ = Type.Rb__tree_Node(d_2_new__right__nodeColor_, ((h).right).key, ((h).right).left, ((h).right).right)
+        d_4_result__nodeColor_: Type.Color
+        if ((h).color) == (Type.Color_Red()):
+            d_4_result__nodeColor_ = Type.Color_Black()
+        elif True:
+            d_4_result__nodeColor_ = Type.Color_Red()
+        result = Type.Rb__tree_Node(d_4_result__nodeColor_, (h).key, d_1_new__left_, d_3_new__right_)
+        return result
+        return result
+
+    @staticmethod
+    def insert__recur(t, insert__key):
+        result: Type.Rb__tree = Type.Rb__tree.default()()
+        if (t).is_Null:
+            result = Type.Rb__tree_Node(Type.Color_Red(), insert__key, Type.Rb__tree_Null(), Type.Rb__tree_Null())
+            return result
+        elif True:
+            d_0_new__t_: Type.Rb__tree
+            d_0_new__t_ = t
+            if (Property.default__.isRed((t).left)) and (Property.default__.isRed((t).right)):
+                out0_: Type.Rb__tree
+                out0_ = default__.flip__color(t)
+                d_0_new__t_ = out0_
+            if (insert__key) > ((d_0_new__t_).key):
+                d_1_r_: Type.Rb__tree
+                out1_: Type.Rb__tree
+                out1_ = default__.insert__recur((d_0_new__t_).right, insert__key)
+                d_1_r_ = out1_
+                result = Type.Rb__tree_Node((d_0_new__t_).color, (d_0_new__t_).key, (d_0_new__t_).left, d_1_r_)
+            elif (insert__key) < ((d_0_new__t_).key):
+                d_2_l_: Type.Rb__tree
+                out2_: Type.Rb__tree
+                out2_ = default__.insert__recur((d_0_new__t_).left, insert__key)
+                d_2_l_ = out2_
+                result = Type.Rb__tree_Node((d_0_new__t_).color, (d_0_new__t_).key, d_2_l_, (d_0_new__t_).right)
+            elif True:
+                result = d_0_new__t_
+            d_3_before__rotate__result_: Type.Rb__tree
+            d_3_before__rotate__result_ = result
+            if Property.default__.rightLeaningRedLink(result):
+                d_4_result__after__rotation_: Type.Rb__tree
+                out3_: Type.Rb__tree
+                out3_ = default__.rotateLeft(d_3_before__rotate__result_)
+                d_4_result__after__rotation_ = out3_
+                result = d_4_result__after__rotation_
+            elif True:
+                pass
+            if Property.default__.doubleLeftRedLink(result):
+                out4_: Type.Rb__tree
+                out4_ = default__.rotateRight(result)
+                result = out4_
+        return result
+        return result
+
+    @staticmethod
+    def makeRootBlack(t):
+        result: Type.Rb__tree = Type.Rb__tree.default()()
+        if (t).is_Node:
+            result = Type.Rb__tree_Node(Type.Color_Black(), (t).key, (t).left, (t).right)
+        elif True:
+            result = Type.Rb__tree_Null()
+        return result
+        return result
+
+    @staticmethod
+    def insert(t, key):
+        root: Type.Rb__tree = Type.Rb__tree.default()()
+        out0_: Type.Rb__tree
+        out0_ = default__.insert__recur(t, key)
+        root = out0_
+        out1_: Type.Rb__tree
+        out1_ = default__.makeRootBlack(root)
+        root = out1_
+        return root
+        return root
+
