main-py/Property.py
@@ -1,0 +1,204 @@
+import sys
+from typing import Callable, Any, TypeVar, NamedTuple
+from math import floor
+from itertools import count
+
+import module_ as module_
+import _dafny as _dafny
+import System_ as System_
+import Type as Type
+
+# Module: Property
+
+class default__:
+    def  __init__(self):
+        pass
+
+    @staticmethod
+    def rootProperty(t):
+        source0_ = t
+        if True:
+            if source0_.is_Null:
+                return True
+        if True:
+            d_0_nodeColor_ = source0_.color
+            return (d_0_nodeColor_) == (Type.Color_Black())
+
+    @staticmethod
+    def nodeColor(t):
+        source0_ = t
+        if True:
+            if source0_.is_Null:
+                return Type.Color_Black()
+        if True:
+            d_0_c_ = source0_.color
+            return d_0_c_
+
+    @staticmethod
+    def Max(left, right):
+        if (left) >= (right):
+            return left
+        elif True:
+            return right
+
+    @staticmethod
+    def BlackHeight(t):
+        source0_ = t
+        if True:
+            if source0_.is_Null:
+                return 1
+        if True:
+            d_0_nodeColor_ = source0_.color
+            d_1_left_ = source0_.left
+            d_2_right_ = source0_.right
+            d_3_leftHeight_ = default__.BlackHeight(d_1_left_)
+            d_4_rightHeight_ = default__.BlackHeight(d_2_right_)
+            d_5_result_ = default__.Max(d_3_leftHeight_, d_4_rightHeight_)
+            if (d_0_nodeColor_) == (Type.Color_Black()):
+                return (d_5_result_) + (1)
+            elif True:
+                return d_5_result_
+
+    @staticmethod
+    def contain(t):
+        source0_ = t
+        if True:
+            if source0_.is_Null:
+                return _dafny.Set({})
+        if True:
+            d_0_key_ = source0_.key
+            d_1_left_ = source0_.left
+            d_2_right_ = source0_.right
+            return ((_dafny.Set({d_0_key_})) | (default__.contain(d_1_left_))) | (default__.contain(d_2_right_))
+
+    @staticmethod
+    def bstProperty(t):
+        source0_ = t
+        if True:
+            if source0_.is_Null:
+                return True
+        if True:
+            d_0_key_ = source0_.key
+            d_1_left_ = source0_.left
+            d_2_right_ = source0_.right
+            def lambda0_(forall_var_0_):
+                d_3_x_: int = forall_var_0_
+                return not ((d_3_x_) in (default__.contain(d_1_left_))) or ((d_3_x_) < (d_0_key_))
+
+            def lambda1_(forall_var_1_):
+                d_4_y_: int = forall_var_1_
+                return not ((d_4_y_) in (default__.contain(d_2_right_))) or ((d_4_y_) > (d_0_key_))
+
+            return (((default__.bstProperty(d_1_left_)) and (default__.bstProperty(d_2_right_))) and (_dafny.quantifier((default__.contain(d_1_left_)).Elements, True, lambda0_))) and (_dafny.quantifier((default__.contain(d_2_right_)).Elements, True, lambda1_))
+
+    @staticmethod
+    def equalContentProperty(t1, t2):
+        return (default__.contain(t1)) == (default__.contain(t2))
+
+    @staticmethod
+    def isRed(t):
+        source0_ = t
+        if True:
+            if source0_.is_Null:
+                return False
+        if True:
+            d_0_nodeColor_ = source0_.color
+            return (d_0_nodeColor_) == (Type.Color_Red())
+
+    @staticmethod
+    def isBlack(t):
+        source0_ = t
+        if True:
+            if source0_.is_Null:
+                return True
+        if True:
+            d_0_nodeColor_ = source0_.color
+            return (d_0_nodeColor_) == (Type.Color_Black())
+
+    @staticmethod
+    def doubleLeftRedLink(h):
+        source0_ = h
+        if True:
+            if source0_.is_Node:
+                d_0_h__nodeColor_ = source0_.color
+                d_1_h__key_ = source0_.key
+                left0 = source0_.left
+                if left0.is_Node:
+                    color0 = left0.color
+                    if color0.is_Red:
+                        d_2_x__key_ = left0.key
+                        left1 = left0.left
+                        if left1.is_Node:
+                            color1 = left1.color
+                            if color1.is_Red:
+                                return True
+        if True:
+            return False
+
+    @staticmethod
+    def goodColor(t):
+        source0_ = t
+        if True:
+            if source0_.is_Null:
+                return True
+        if True:
+            d_0_c_ = source0_.color
+            d_1_l_ = source0_.left
+            d_2_r_ = source0_.right
+            if (d_0_c_) == (Type.Color_Red()):
+                return ((default__.nodeColor(d_1_l_)) == (Type.Color_Black())) and ((default__.nodeColor(d_2_r_)) == (Type.Color_Black()))
+            elif True:
+                return not ((default__.nodeColor(d_2_r_)) == (Type.Color_Red())) or ((default__.nodeColor(d_1_l_)) == (Type.Color_Red()))
+
+    @staticmethod
+    def rightLeaningRedLink(t):
+        source0_ = t
+        if True:
+            if source0_.is_Node:
+                left0 = source0_.left
+                if left0.is_Null:
+                    right0 = source0_.right
+                    if right0.is_Node:
+                        color0 = right0.color
+                        if color0.is_Red:
+                            return True
+        if True:
+            if source0_.is_Node:
+                left1 = source0_.left
+                if left1.is_Node:
+                    color1 = left1.color
+                    if color1.is_Black:
+                        right1 = source0_.right
+                        if right1.is_Node:
+                            color2 = right1.color
+                            if color2.is_Red:
+                                return True
+        if True:
+            return False
+
+    @staticmethod
+    def strongLLRB(t):
+        source0_ = t
+        if True:
+            if source0_.is_Null:
+                return True
+        if True:
+            d_0_c_ = source0_.color
+            d_1_k_ = source0_.key
+            d_2_l_ = source0_.left
+            d_3_r_ = source0_.right
+            return ((((default__.strongLLRB(d_2_l_)) and (default__.strongLLRB(d_3_r_))) and ((default__.BlackHeight(d_2_l_)) == (default__.BlackHeight(d_3_r_)))) and (default__.bstProperty(t))) and (default__.goodColor(t))
+
+    @staticmethod
+    def weakLLRB(t):
+        source0_ = t
+        if True:
+            if source0_.is_Null:
+                return True
+        if True:
+            d_0_c_ = source0_.color
+            d_1_k_ = source0_.key
+            d_2_l_ = source0_.left
+            d_3_r_ = source0_.right
+            return ((((default__.strongLLRB(d_2_l_)) and (default__.strongLLRB(d_3_r_))) and ((default__.BlackHeight(d_2_l_)) == (default__.BlackHeight(d_3_r_)))) and (default__.bstProperty(t))) and (not ((default__.nodeColor(d_3_r_)) == (Type.Color_Red())) or ((default__.nodeColor(d_2_l_)) == (Type.Color_Red())))
+
