main-py/Type.py
@@ -1,0 +1,74 @@
+import sys
+from typing import Callable, Any, TypeVar, NamedTuple
+from math import floor
+from itertools import count
+
+import module_ as module_
+import _dafny as _dafny
+import System_ as System_
+
+# Module: Type
+
+
+class Color:
+    @_dafny.classproperty
+    def AllSingletonConstructors(cls):
+        return [Color_Red(), Color_Black()]
+    @classmethod
+    def default(cls, ):
+        return lambda: Color_Red()
+    def __ne__(self, __o: object) -> bool:
+        return not self.__eq__(__o)
+    @property
+    def is_Red(self) -> bool:
+        return isinstance(self, Color_Red)
+    @property
+    def is_Black(self) -> bool:
+        return isinstance(self, Color_Black)
+
+class Color_Red(Color, NamedTuple('Red', [])):
+    def __dafnystr__(self) -> str:
+        return f'Type.Color.Red'
+    def __eq__(self, __o: object) -> bool:
+        return isinstance(__o, Color_Red)
+    def __hash__(self) -> int:
+        return super().__hash__()
+
+class Color_Black(Color, NamedTuple('Black', [])):
+    def __dafnystr__(self) -> str:
+        return f'Type.Color.Black'
+    def __eq__(self, __o: object) -> bool:
+        return isinstance(__o, Color_Black)
+    def __hash__(self) -> int:
+        return super().__hash__()
+
+
+class Rb__tree:
+    @classmethod
+    def default(cls, ):
+        return lambda: Rb__tree_Null()
+    def __ne__(self, __o: object) -> bool:
+        return not self.__eq__(__o)
+    @property
+    def is_Null(self) -> bool:
+        return isinstance(self, Rb__tree_Null)
+    @property
+    def is_Node(self) -> bool:
+        return isinstance(self, Rb__tree_Node)
+
+class Rb__tree_Null(Rb__tree, NamedTuple('Null', [])):
+    def __dafnystr__(self) -> str:
+        return f'Type.Rb_tree.Null'
+    def __eq__(self, __o: object) -> bool:
+        return isinstance(__o, Rb__tree_Null)
+    def __hash__(self) -> int:
+        return super().__hash__()
+
+class Rb__tree_Node(Rb__tree, NamedTuple('Node', [('color', Any), ('key', Any), ('left', Any), ('right', Any)])):
+    def __dafnystr__(self) -> str:
+        return f'Type.Rb_tree.Node({_dafny.string_of(self.color)}, {_dafny.string_of(self.key)}, {_dafny.string_of(self.left)}, {_dafny.string_of(self.right)})'
+    def __eq__(self, __o: object) -> bool:
+        return isinstance(__o, Rb__tree_Node) and self.color == __o.color and self.key == __o.key and self.left == __o.left and self.right == __o.right
+    def __hash__(self) -> int:
+        return super().__hash__()
+
