main-py/module_.py
@@ -1,0 +1,63 @@
+import sys
+from typing import Callable, Any, TypeVar, NamedTuple
+from math import floor
+from itertools import count
+
+import module_ as module_
+import _dafny as _dafny
+import System_ as System_
+import Type as Type
+import Property as Property
+import Lem as Lem
+import Operations as Operations
+
+# Module: module_
+
+class default__:
+    def  __init__(self):
+        pass
+
+    @staticmethod
+    def Pad(n):
+        d_0___accumulator_ = _dafny.SeqWithoutIsStrInference([])
+        while True:
+            with _dafny.label():
+                if (n) == (0):
+                    return (d_0___accumulator_) + (_dafny.SeqWithoutIsStrInference(map(_dafny.CodePoint, "")))
+                elif True:
+                    d_0___accumulator_ = (d_0___accumulator_) + (_dafny.SeqWithoutIsStrInference(map(_dafny.CodePoint, " ")))
+                    in0_ = (n) - (1)
+                    n = in0_
+                    raise _dafny.TailCall()
+                break
+
+    @staticmethod
+    def PrintTree(t, indent):
+        if (t) == (Type.Rb__tree_Null()):
+            _dafny.print((default__.Pad(indent)).VerbatimString(False))
+            _dafny.print((_dafny.SeqWithoutIsStrInference(map(_dafny.CodePoint, "·\n"))).VerbatimString(False))
+        elif True:
+            default__.PrintTree((t).right, (indent) + (4))
+            _dafny.print((default__.Pad(indent)).VerbatimString(False))
+            _dafny.print(((_dafny.SeqWithoutIsStrInference(map(_dafny.CodePoint, "R")) if ((t).color) == (Type.Color_Red()) else _dafny.SeqWithoutIsStrInference(map(_dafny.CodePoint, "B")))).VerbatimString(False))
+            _dafny.print((_dafny.SeqWithoutIsStrInference(map(_dafny.CodePoint, "("))).VerbatimString(False))
+            _dafny.print(_dafny.string_of((t).key))
+            _dafny.print((_dafny.SeqWithoutIsStrInference(map(_dafny.CodePoint, ")\n"))).VerbatimString(False))
+            default__.PrintTree((t).left, (indent) + (4))
+
+    @staticmethod
+    def Main(noArgsParameter__):
+        d_0_t_: Type.Rb__tree
+        d_0_t_ = Type.Rb__tree_Null()
+        d_1_keys_: _dafny.Seq
+        d_1_keys_ = _dafny.SeqWithoutIsStrInference([10, 7, 18, 2, 8, 15, 25, 1, 3])
+        d_2_i_: int
+        d_2_i_ = 0
+        while (d_2_i_) < (len(d_1_keys_)):
+            out0_: Type.Rb__tree
+            out0_ = Operations.default__.insert(d_0_t_, (d_1_keys_)[d_2_i_])
+            d_0_t_ = out0_
+            d_2_i_ = (d_2_i_) + (1)
+        _dafny.print((_dafny.SeqWithoutIsStrInference(map(_dafny.CodePoint, "RedBlack tree after inserts:\n"))).VerbatimString(False))
+        default__.PrintTree(d_0_t_, 0)
+
